Source/IntegrationTests/TestFiles/LitTests/LitTest/invariants/TempInvariantBreaking.dfy
@@ -1,4 +1,4 @@
-// RUN: %verify --type-system-refresh --check-invariants "%s" > "%t"
+// RUN: %verify --type-system-refresh --check-invariants --reads-clauses-on-methods "%s" > "%t"
 // RUN: %diff "%s.expect" "%t"
 
 class C {
@@ -18,11 +18,22 @@ class C {
      x := 0; // temporarily breaking the invariant outside the constructor is allowed
      //UseInvariant(this); // error: invariant doesn't hold here (force checked, since this is open)
      var me := this;
-     //UseInvariant(me); //  error: same as above (this can be copied as much as you want)
+     MethodReadsNothing();
+     var _ := FunctionReadsNothing();
+     //var _ := me.InstanceUsesInvariant() + 2; //  error: same as above (this can be copied as much as you want)
      x := 1;
   }
+  
+  // invariant assumed here
+  function InstanceUsesInvariant(): int reads this {
+    1 / x
+  }
+  
+  // NB: invariant is not assumed/asserted in these
+  static method MethodReadsNothing() reads {} {}
+  opaque predicate FunctionReadsNothing() reads {} { true }
  
-  static method UseInvariant(c: C) 
+  static method UseInvariant(c: C)
   {
     var y := 3 / c.x;
   }
